PsBool.v
@@ -26,10 +26,12 @@ Definition instfalse : inst := instnop.
 Definition insttrue : inst := instswap.
 
 Lemma eval_insttrue : insttrue_spec insttrue.
+Proof.
   repeat intro ; evalauto.
 Qed.
 
 Lemma eval_instfalse : instfalse_spec instfalse.
+Proof.
   repeat intro ; evalauto.
 Qed.
 
@@ -42,6 +44,7 @@ Definition instnot : inst := instpair (instpush instswap) instcons.
 Lemma instnot_proof : forall b i1 vs cs, instbool_spec b i1 ->
   exists i2 : inst, instbool_spec (negb b) i2 /\
   (i1 :: vs, instnot :: cs) |=>* (i2 :: vs, cs).
+Proof.
   intros ; evalauto ; destruct b ;
     repeat intro ; evalauto ; evalpartial H ; evalauto.
 Qed.
@@ -62,6 +65,7 @@ Definition instif : inst := instseq
 Lemma eval_instif : forall b i1 i2 i3 vs cs,
   instbool_spec b i1 -> (i3 :: i2 :: i1 :: vs, instif :: cs) |=>*
     ((if b then i2 else i3) :: vs, cs).
+Proof.
   intros.
   destruct b ; evalauto ; evalpartial H ; evalauto.
 Qed.
@@ -71,6 +75,7 @@ Definition instexecif : inst := instpair instif instexec.
 Lemma eval_instexecif : forall b i1 i2 i3 vs cs,
   instbool_spec b i1 -> (i3 :: i2 :: i1 :: vs, instexecif :: cs) |=>*
     (vs, (if b then i2 else i3) :: cs).
+Proof.
   intros.
   destruct b ; evalauto ; evalpartial H ; evalauto.
 Qed.
@@ -85,6 +90,7 @@ Lemma instxor_proof : forall b1 b2 i1 i2 vs cs,
   instbool_spec b1 i1 -> instbool_spec b2 i2 ->
     exists i3 : inst, instbool_spec (xorb b1 b2) i3 /\
     (i2 :: i1 :: vs, instxor :: cs) |=>* (i3 :: vs, cs).
+Proof.
   intros ; evalauto ; destruct b1, b2 ; repeat intro ;
     evalauto ; evalpartial H ; evalpartial H0 ; evalauto.
 Qed.
